elo-coq/Map.v
@@ -1,30 +1,36 @@
 From Coq Require Import Strings.String.
 
 Inductive map (A : Type) : Type :=
-  | nil
-  | cons (k : string) (v : A) (m : map A)
+  | map_nil
+  | map_cons (k : string) (v : A) (m : map A)
   .
 
-Definition empty {A} := nil A.
+Definition empty {A} := map_nil A.
 
 Fixpoint update {A} (m : map A) k v :=
   match m with
-  | nil _ => cons A k v (nil A)
-  | cons _ k' v' m' =>
+  | map_nil _ => map_cons A k v (map_nil A)
+  | map_cons _ k' v' m' =>
       if eqb k k'
-        then cons A k  v  (update m' k v)
-        else cons A k' v' (update m' k v)
+        then map_cons A k  v  (update m' k v)
+        else map_cons A k' v' (update m' k v)
   end.
-
-Local Definition update' {A} m k v := cons A k v m.
 
 Fixpoint lookup {A} m k : option A :=
   match m with
-  | nil _ => None
-  | cons _ k' v m' => if eqb k' k then Some v else lookup m' k
+  | map_nil _ => None
+  | map_cons _ k' v m' => if eqb k' k then Some v else lookup m' k
   end.
 
-Theorem update_equivalence : forall {A} (m : map A) k v id,
+(* m includes m' *)
+Local Definition includes' {A} (m m' : map A) :=
+  forall k v, lookup m' k = Some v -> lookup m k = Some v.
+
+Infix "includes" := includes' (at level 50, left associativity).
+
+Local Definition update' {A} m k v := map_cons A k v m.
+
+Local Theorem update_equivalence : forall {A} (m : map A) k v id,
   lookup (update m k v) id = lookup (update' m k v) id.
 Proof.
   intros *. unfold update', update.
@@ -37,62 +43,40 @@ Proof.
     destruct (eqb k id) eqn:E3; trivial; discriminate.
 Qed.
 
-Corollary update_equivalence_impl : forall {A} (m : map A) k k' v v',
-  lookup (update m k' v') k = Some v <-> lookup (update' m k' v') k = Some v.
+Local Lemma lookup_update_k_eq' : forall {A} (m : map A) k v,
+  lookup (update' m k v) k = Some v.
 Proof.
-  intros *. rewrite update_equivalence. split; trivial.
+  intros. simpl. rewrite String.eqb_refl. reflexivity.
 Qed.
 
-Lemma lookup_update_k_eq : forall {A} (m : map A) k v,
-  lookup (update m k v) k = Some v.
-Proof.
-  intros. rewrite update_equivalence.
-  simpl. rewrite String.eqb_refl. reflexivity.
-Qed.
-
-Lemma lookup_update_k_neq : forall {A} (m : map A) k k' v,
+Local Lemma lookup_update_k_neq' : forall {A} (m : map A) k k' v,
   k' <> k ->
-  lookup (update m k' v) k = lookup m k.
+  lookup (update' m k' v) k = lookup m k.
 Proof.
-  intros * H. rewrite update_equivalence.
-  simpl. destruct eqb eqn:E; trivial.
+  intros * H. simpl. destruct eqb eqn:E; trivial.
   apply String.eqb_eq in E. contradiction.
 Qed.
 
-(* m includes m' *)
-Local Definition includes_definition {A} (m m' : map A) :=
-  forall k v, lookup m' k = Some v -> lookup m k = Some v.
-
-Infix "includes" := includes_definition (at level 50, left associativity).
-
-Lemma update_preserves_inclusion : forall {A} (m m' : map A) k v,
+Local Lemma update_preserves_inclusion' : forall {A} (m m' : map A) k v,
   m includes m' ->
-  (update m k v) includes (update m' k v).
+  (update' m k v) includes (update' m' k v).
 Proof.
-  intros * ? k' ? H.
-  unfold includes_definition in *. 
-  rewrite update_equivalence in *.
-  unfold lookup, update' in *.
-  destruct m; destruct (eqb k k'); eauto.
+  intros *. unfold includes', lookup, update'.
+  destruct m; intros * ? k'; destruct (eqb k k'); eauto.
 Qed.
 
-Lemma update_overwrite : forall {A} (m : map A) k v v',
-  (update m k v) includes (update (update m k v') k v).
+Local Lemma update_overwrite' : forall {A} (m : map A) k v v',
+  (update' m k v) includes (update' (update' m k v') k v).
 Proof.
-  intros *. unfold includes_definition. intros k' ?.
-  rewrite 2 update_equivalence.
-  unfold lookup, update'.
-  destruct m; intros H; destruct (eqb k k') eqn:E; trivial;
-  rewrite update_equivalence in H;
-  unfold lookup, update' in H;
-  rewrite E in H; assumption.
+  unfold includes', lookup, update'. intros ? ? ? ? ? k' ?.
+  destruct m; intros H; destruct (eqb k k'); assumption.
 Qed.
 
-Lemma update_permutation : forall {A} (m : map A) k1 k2 v1 v2,
+Local Lemma update_permutation' : forall {A} (m : map A) k1 k2 v1 v2,
   k1 <> k2 ->
   (update' (update' m k1 v1) k2 v2) includes (update' (update' m k2 v2) k1 v1).
 Proof.
-  intros * Hneq. unfold includes_definition.
+  intros * Hneq. unfold includes'.
   induction m as [| ? ? ? IH]; intros k' v'.
   - unfold update', lookup.
     destruct (eqb k1 k') eqn:E1; trivial.
@@ -103,18 +87,93 @@ Proof.
     destruct (eqb k1 k') eqn:E1.
     + apply eqb_eq in E1. subst.
       destruct (eqb k2 k') eqn:E2.
-      * apply eqb_eq in E2. subst. rewrite 2 lookup_update_k_eq in *. trivial.
+      * apply eqb_eq in E2. subst. rewrite 2 lookup_update_k_eq' in *. trivial.
       * apply eqb_neq in E2.
-        rewrite (lookup_update_k_neq _ _ _ _ E2).
-        rewrite 2 lookup_update_k_eq in *.
+        rewrite (lookup_update_k_neq' _ _ _ _ E2).
+        rewrite 2 lookup_update_k_eq' in *.
         intros H. specialize (IH H).
         assumption.
     + apply eqb_neq in E1.
-      rewrite (lookup_update_k_neq _ _ _ _ E1) in *.
+      rewrite (lookup_update_k_neq' _ _ _ _ E1) in *.
       destruct (eqb k2 k') eqn:E2.
-      * apply eqb_eq in E2. subst. rewrite 2 lookup_update_k_eq. trivial.
+      * apply eqb_eq in E2. subst. rewrite 2 lookup_update_k_eq'. trivial.
       * apply eqb_neq in E2.
-        rewrite 2 (lookup_update_k_neq _ _ _ _ E2) in *.
+        rewrite 2 (lookup_update_k_neq' _ _ _ _ E2) in *.
+        rewrite (lookup_update_k_neq' _ _ _ _ E1) in *.
+        trivial.
+Qed.
+
+Corollary lookup_update_k_eq : forall {A} (m : map A) k v,
+  lookup (update m k v) k = Some v.
+Proof.
+  intros. rewrite update_equivalence. auto using lookup_update_k_eq'.
+Qed.
+
+Corollary lookup_update_k_neq : forall {A} (m : map A) k k' v,
+  k' <> k ->
+  lookup (update m k' v) k = lookup m k.
+Proof.
+  intros * H. rewrite update_equivalence. auto using lookup_update_k_neq'.
+Qed.
+
+Corollary update_preserves_inclusion : forall {A} (m m' : map A) k v,
+  m includes m' ->
+  (update m k v) includes (update m' k v).
+Proof.
+  intros. unfold includes'. intros *.
+  rewrite 2 update_equivalence. apply update_preserves_inclusion'. assumption.
+Qed.
+
+Lemma update_overwrite : forall {A} (m : map A) k v v',
+  (update m k v) includes (update (update m k v') k v).
+Proof.
+  unfold includes'. intros ? ? ? ? ? k' ?.
+  rewrite 2 update_equivalence.
+  unfold lookup, update'.
+  destruct m; intros H; destruct (eqb k k') eqn:E; trivial;
+  fold (@lookup A) in H; rewrite update_equivalence in H;
+  unfold lookup, update' in H; rewrite E in H; assumption.
+Qed.
+
+Lemma update_permutation : forall {A} (m : map A) k1 k2 v1 v2,
+  k1 <> k2 ->
+  (update (update m k1 v1) k2 v2) includes (update (update m k2 v2) k1 v1).
+Proof.
+  intros * Hneq. unfold includes'.
+  intros k v. rewrite 2 update_equivalence.
+  generalize dependent v. generalize dependent k.
+  induction m as [| ? ? ? IH]; intros k' v'.
+  - unfold update', lookup.
+    destruct (eqb k1 k') eqn:E1; destruct (eqb k2 k') eqn:E2.
+    + apply eqb_eq in E1, E2. subst. contradiction.
+    + apply eqb_eq in E1. subst.
+      fold (@lookup A). rewrite update_equivalence.
+      unfold update', lookup. rewrite eqb_refl. trivial.
+    + apply eqb_eq in E2. subst.
+      fold (@lookup A). rewrite update_equivalence.
+      unfold update', lookup. rewrite eqb_refl. trivial.
+    + fold (@lookup A). rewrite 2 update_equivalence.
+      unfold update', lookup. rewrite E1, E2. trivial.
+  - specialize (IH k' v').
+    destruct (eqb k1 k') eqn:E1.
+    + apply eqb_eq in E1. subst.
+      destruct (eqb k2 k') eqn:E2.
+      * apply eqb_eq in E2. subst. rewrite 2 lookup_update_k_eq' in *. trivial.
+      * apply eqb_neq in E2.
+        rewrite (lookup_update_k_neq' _ _ _ _ E2).
+        rewrite update_equivalence.
+        rewrite 2 lookup_update_k_eq' in *.
+        trivial.
+    + apply eqb_neq in E1.
+      rewrite (lookup_update_k_neq' _ _ _ _ E1) in *.
+      destruct (eqb k2 k') eqn:E2.
+      * apply eqb_eq in E2. subst.
+        rewrite update_equivalence.
+        rewrite 2 lookup_update_k_eq'.
+        trivial.
+      * apply eqb_neq in E2.
+        rewrite update_equivalence.
+        rewrite 2 (lookup_update_k_neq' _ _ _ _ E2) in *.
         rewrite (lookup_update_k_neq _ _ _ _ E1) in *.
         trivial.
 Qed.
